module TermRed2 where

open import Data.Zero
open import Function
open import Function.Extensionality
open import Relation.Binary.NP
open import Relation.Binary.PropositionalEquality.NP
  hiding ([_])
  renaming (_â‰¡_ to _==_; _â‰—_ to _~_)

open import Sketch5
open import Terms

open Term-Structure Tm-Monad

-- Not used yet
mutual
    -- Neutral forms
    data Neu {Î±} : Tm Î± â†’ Type where
      var  : âˆ€ x â†’ Neu (var x)
      _$$_ : âˆ€ {t u} â†’ Neu t â†’ Nrm u â†’ Neu (t $$ u)

    -- Normal forms
    data Nrm {Î±} : Tm Î± â†’ Type where
      Æ›_  : {t : Tm (Î± â‡‘)} â†’ Nrm t â†’ Nrm (Æ› t)
      neu : âˆ€ {t} â†’ Neu t â†’ Nrm t
      

data Value {Î±} : Tm Î± â†’ Type where
  Æ›_ : âˆ€ t â†’ Value (Æ› t)

infix 2 _âŸ¶_
data _âŸ¶_ {Î±} : (t v : Tm Î±) â†’ Type where
  Î²    : âˆ€ {t t' u vu v}
           (rt : t âŸ¶ Æ› t')
           (ru : u âŸ¶ vu)
           (rv : [ 0â‰” vu ] t' âŸ¶ v)
         â†’ t $$ u âŸ¶ v
  Æ›_   : âˆ€ t â†’ Æ› t âŸ¶ Æ› t

âŸ¶-Value : âˆ€ {Î±} {t v : Tm Î±} â†’ t âŸ¶ v â†’ Value v
âŸ¶-Value (Î² r râ‚ râ‚‚) = âŸ¶-Value râ‚‚
âŸ¶-Value (Æ› t) = Æ› t

âŸ¶-trans : âˆ€ {Î±} â†’ Transitive (_âŸ¶_ {Î±})
âŸ¶-trans (Î² rt ru rv) r = Î² rt ru (âŸ¶-trans rv r)
âŸ¶-trans (Æ› t) q = q

module âŸ¶-Reasoning {Î± : World} where
  infix  2 finally
  infixr 2 _âŸ¶âŸ¨_âŸ©_

  _âŸ¶âŸ¨_âŸ©_ : âˆ€ x {y z : Tm Î±} â†’ x âŸ¶ y â†’ y âŸ¶ z â†’ x âŸ¶ z
  _ âŸ¶âŸ¨ xâ‰ˆy âŸ© yâ‰ˆz = âŸ¶-trans xâ‰ˆy yâ‰ˆz

  -- When there is no reflexivty available this
  -- combinator can be used to end the reasoning.
  finally : âˆ€ (x y : Tm Î±) â†’ x âŸ¶ y â†’ x âŸ¶ y
  finally _ _ xâ‰ˆy = xâ‰ˆy

  syntax finally x y xâ‰ˆy = x âŸ¶âŸ¨ xâ‰ˆy âŸ©âˆŽ y âˆŽ

module _ {Î± : World} where

    _â‰ˆ_ : âˆ€ (t u : Tm Î±) â†’ Type
    t â‰ˆ u = âˆ€ {v} â†’ t âŸ¶ v â†’ u âŸ¶ v

    â‰ˆ-refl : Reflexive _â‰ˆ_
    â‰ˆ-refl = id

    â‰ˆ-trans : Transitive _â‰ˆ_
    â‰ˆ-trans p q = q âˆ˜ p

    module â‰ˆ-Reasoning = Refl-Trans-Reasoning _â‰ˆ_ â‰ˆ-refl â‰ˆ-trans

    {-
    Î²-â‰ˆ : âˆ€ {t} {u : Tm Î±} â†’ [ 0â‰” u ] t â‰ˆ (Æ› t $$ u)
    Î²-â‰ˆ = Î² (Æ› _) {!!}
    -}

    â‰ˆ-reflexive : âˆ€ {t u : Tm Î±} -> (t == u) -> (t â‰ˆ u)
    â‰ˆ-reflexive refl x = x

    {-
    âŸ¶-â‰ˆ : âˆ€ {t u : Tm Î±} -> t âŸ¶ u â†’ u â‰ˆ t
    âŸ¶-â‰ˆ r r' = âŸ¶-trans r r'
    -}

infix 2 _âŸ¶Â°_
_âŸ¶Â°_ : âˆ€ {Î± Î²}(s s' : Î± â‡¶ Î²) â†’ Type
s âŸ¶Â° s' = âˆ€ x â†’ s x âŸ¶ s' x

0â‰”âŸ¶Â° : âˆ€ {M v : Tm ðŸ˜} (r : M âŸ¶ v) â†’ 0â‰” M âŸ¶Â° 0â‰” v
0â‰”âŸ¶Â° r (old ())
0â‰”âŸ¶Â° r (new .â™¦) = r

{-
module _ {{_ : FunExt}} where
    open â‰¡-Reasoning

    postulate mapâŸ¶ : âˆ€ {a b} {f : a -> b} {f' : a -> b} (f= : f ~ f') {t u : Tm a} -> (t âŸ¶ u) -> f <$> t âŸ¶ f' <$> u
    {-
    mapâŸ¶ f= noop = {!â‰ˆ-reflexive (ap (Î» f â†’ f <$> _) (Î»= (!_ âˆ˜ f=))) noop!}
    mapâŸ¶ {f = f} {f'} f= (Î² {t} {u} {v} r) = Î² (tr id (! pf) (mapâŸ¶ f= r))
      where pf = (0â‰” (f <$> u) =<< (mapâ‡‘ f <$> t) âŸ¶ f' <$> v)
               â‰¡âŸ¨ ap (Î» x â†’ x âŸ¶ f' <$> v) (=<<-<$> t) âŸ©
                 ((0â‰” (f <$> u) âˆ˜ mapâ‡‘ f) =<< t âŸ¶ f' <$> v)
               â‰¡âŸ¨ ap (Î» x â†’ x =<< t âŸ¶ f' <$> v) (Î»= (0â‰”-map f u)) âŸ©
                 (map f âˆ˜ 0â‰” u =<< t âŸ¶ f' <$> v)
               â‰¡âŸ¨ ap (Î» x â†’ x âŸ¶ f' <$> v) (! <$>-=<< t) âŸ©
                 (f <$> 0â‰” u =<< t âŸ¶ f' <$> v)
               âˆŽ
    mapâŸ¶ f= (r1 $$ r2) = mapâŸ¶ f= r1 $$ mapâŸ¶ f= r2
    mapâŸ¶ f= (Æ› r) = Æ› mapâŸ¶ (mapâ‡‘= f=) r
    -}

    extâŸ¶ : âˆ€ {a b} {s s' : a â‡¶ b} -> (s âŸ¶Â° s') -> (ext s âŸ¶Â° ext s')
    extâŸ¶ s= (old x) = mapâŸ¶ (Î» xâ‚ â†’ refl) (s= x)
    extâŸ¶ s= (new .â™¦) = {!!}

    substâŸ¶Â°1 : âˆ€ {a b} {s s' : a â‡¶ b} -> (s âŸ¶Â° s') -> substT s âŸ¶Â° substT s'
    substâŸ¶Â°1 s= (var x)  = s= x
    substâŸ¶Â°1 s= (Æ› M)    = Æ› (substâŸ¶Â°1 (extâŸ¶ s=) M)
    substâŸ¶Â°1 s= (M $$ N) = Î² {!substâŸ¶Â°1 s= M!} {!substâŸ¶Â°1 s= N!}

    substâŸ¶ : âˆ€ {a b} {M M' : Tm a} {s s' : a â‡¶ b} â†’ (M âŸ¶ M') â†’ (s âŸ¶Â° s') â†’ M >>= s âŸ¶ M' >>= s'
    substâŸ¶ {M' = M'} {s} {s'} (Î² {t} {u} {v} r1 r2) x =
      Î² (substâŸ¶ r1 x) (tr (Î» tâ‚ â†’ tâ‚ âŸ¶ M' >>= s') (! bind-assoc' u ) (substâŸ¶ {!r2!} {!!}))
      -- {!(â‰ˆ-reflexive (bind-assoc' t âˆ™ ! ap (_>>=_ t) (Î»= subst0-ext) âˆ™ ! bind-assoc' t) (substâŸ¶ r1 x)) ?!}
    {-
    substâŸ¶ {M = M} noop x = {!substâŸ¶Â°1 x M!}
    substâŸ¶ (Î² {t} r1) x =
      Î² (â‰ˆ-reflexive (bind-assoc' t âˆ™ ! ap (_>>=_ t) (Î»= subst0-ext) âˆ™ ! bind-assoc' t) (substâŸ¶ r1 x))
    substâŸ¶ (r1 $$ r2) x = substâŸ¶ r1 x $$ substâŸ¶ r2 x 
    -}
    substâŸ¶ (Æ› r1) x = Æ› substâŸ¶ r1 (extâŸ¶ x)

    subst-lemma : âˆ€ {a} {M v : Tm a} {N v' : ScopeF Tm a} (rM : M âŸ¶ v) (rN : N âŸ¶ v') -> [ 0â‰” M ] N âŸ¶ [ 0â‰” v ] v'
    subst-lemma rM rN = substâŸ¶ rN (0â‰”âŸ¶Â° rM)
-- -}
-- -}
-- -}
-- -}
